---
title: "midterm sample solution"
excerpt: "'열역학 및 통계물리' 과목의 중간고사 해설입니다."
tags: syllabus physics thermodynamics statistics
header:
  teaser: https://drive.google.com/thumbnail?id=1weJXGiV5u1I0FHW_79NqQ9ZQpWEBKKCZ&sz=w1000
---

## 1.
(a)
(i) Clausius theorem : $$ \oint \frac{đQ}{T} \le 0 \quad (= : \text{rev.}) $$

(ii) Entropy

if I and II are reversible

[Diagram: Cycle between points A and B]

$$ \oint \frac{đQ}{T} = \int_{I} \frac{đQ}{T} + \int_{-II} \frac{đQ}{T} = 0 $$

$$ \Rightarrow \quad \int_{I} \frac{đQ}{T} = \int_{II} \frac{đQ}{T} \quad \text{for arb. I and II} $$

$\therefore$ Path independent.

Thus. $$ S_I = S_{II} = \int_{A}^{B} \frac{đQ}{T} \equiv \int_{A}^{B} dS = S_B - S_A $$

$$ \text{entropy} \doteq dS = \frac{đQ}{T} $$

(iii) If path I is irreversible,

$$ \int_{I} \frac{đQ}{T} + \int_{-II} \frac{đQ}{T} \le 0 \quad \Rightarrow \quad \int_{II} \frac{đQ}{T} \ge \int_{I} \frac{đQ}{T} $$

Since II is reversible, $$ S_B - S_A \ge \int_{I} \frac{đQ}{T} $$

For an isolated system, and let I is a physical path

$$ \Rightarrow \quad \underline{\Delta S \ge 0} $$

***

(b) 1st Law

$$ dU = đQ + đW $$

*   $dU$: internal energy change
*   $đQ$: heat absorbed
*   $đW$: work done on the sys.

reversible : $đQ = TdS$ , quasi-static $đW = -pdV$ ☑

$$ \Rightarrow \quad \underline{TdS = dU + pdV} $$

---

(e)

<table style="border: 1px solid black; width: 300px;">
  <tr>
    <td style="padding: 20px; vertical-align: top;">
      T, P
      <div style="border: 1px solid black; border-radius: 50%; width: 50px; height: 50px; display: flex; justify-content: center; align-items: center; margin: 10px;">
        sys
      </div>
    </td>
  </tr>
</table>

$\leftarrow$ reservoir $(T_R=T, P_R=P)$

$\delta S_R = \frac{1}{T_R}\delta U_R + \frac{P_R}{T_R}\delta V_R$

then,

$\delta S_{tot} = \underset{\substack{\uparrow \\ \text{system}}}{\delta S} - \frac{1}{T}\delta U - \frac{P}{T}\delta V \quad (\delta U + \delta U_R = 0, \delta V + \delta V_R = 0)$

$\Rightarrow \quad \delta S_{tot} = -\frac{1}{T} [\delta U - T\delta S + p\delta V]$

$= -\frac{1}{T}\delta G \geq 0$

Thus $\underline{\delta G \leq 0}$ for a given $(T, P)$

Using $dG = -SdT + VdP \Rightarrow \left[ \begin{array}{l} -S = (\frac{\partial G}{\partial T})_P \\ V = (\frac{\partial G}{\partial P})_T \end{array} \right.$

Maxwell relation : $-(\frac{\partial S}{\partial P})_T = (\frac{\partial V}{\partial T})_P$

---

## 2.

(a)
$dU = (\frac{\partial U}{\partial T})_V dT + (\frac{\partial U}{\partial V})_T dV \qquad || \ U \equiv U(T,V)$
$dS = (\frac{\partial S}{\partial T})_V dT + (\frac{\partial S}{\partial V})_T dV \qquad || \ S \equiv S(T,V)$

Using $TdS = dU + pdV$ (1st and 2nd laws)

$T(\frac{\partial S}{\partial T})_V dT + T(\frac{\partial S}{\partial V})_T dV = (\frac{\partial U}{\partial T})_V dT + (\frac{\partial U}{\partial V})_T dV$
$\phantom{T(\frac{\partial S}{\partial T})_V dT + T(\frac{\partial S}{\partial V})_T dV =} + \ pdV$

$\Rightarrow \left[ \begin{array}{l} (\frac{\partial U}{\partial T})_V = T (\frac{\partial S}{\partial T})_V \\ (\frac{\partial U}{\partial V})_T = T \underbrace{(\frac{\partial S}{\partial V})_T}_{\mathclap{\substack{\downarrow \\ \text{Maxwell relation}}}} - P \end{array} \right.$

$\phantom{\Rightarrow \left[ \begin{array}{l} (\frac{\partial U}{\partial T})_V \end{array} \right.} = T \underset{= P/T}{(\frac{\partial P}{\partial T})_V} - P = \underline{\underline{0}}_{,,} \quad || \ PV = Nk_BT$

---

(b) **initial** $\quad \longrightarrow \quad$ **final**
[Box with left half shaded] $\quad \longrightarrow \quad$ [Box fully shaded with diagonal lines]

It's an ideal gas. $\rightarrow U \equiv U(T) = const. \therefore T_i = T_f$
To compute $\Delta S$, connect initial and final states with an isothermal process.

$\Rightarrow \quad TdS = pdV = \frac{Nk_B T}{V} dV$ $\quad \xrightarrow{\text{integrate?}}$

$\underline{\Delta S = N k_B \ln 2}$

---

let
(c) $U \equiv U(T,V) \quad \Rightarrow \quad \underline{\underline{dU = \left(\frac{\partial U}{\partial T}\right)_V dT + \left(\frac{\partial U}{\partial V}\right)_T dV = 0}}$

Thus.
$$ \left(\frac{\partial T}{\partial V}\right)_U = - \frac{\left(\frac{\partial U}{\partial V}\right)_T}{\left(\frac{\partial U}{\partial T}\right)_V} \quad (\text{chain rule}) $$

$$ \Rightarrow \quad \left(\frac{\partial T}{\partial V}\right)_U = - \frac{1}{C_V} \left(\frac{\partial U}{\partial V}\right)_T $$

from (a).
$$ \left(\frac{\partial U}{\partial V}\right)_T = T \left(\frac{\partial P}{\partial T}\right)_V - P $$

$$ \therefore \quad \Delta T = \int_{V_i}^{V_f} \left(\frac{\partial T}{\partial V}\right)_U dV = - \int_{V_i}^{V_f} \frac{1}{C_V} \left( T \left(\frac{\partial P}{\partial T}\right)_V - P \right) dV $$

---

for a vdW gas , $P = \frac{N k_B T}{V - Nb} - \frac{a N^2}{V^2}$

$\left(\frac{\partial P}{\partial T}\right)_{V,N} = \frac{N k_B}{V - Nb}$ , thus $T \left(\frac{\partial P}{\partial T}\right)_V - P = \frac{a N^2}{V^2} > 0$

$\Rightarrow \quad \underline{\Delta T < 0}$ $\quad$ (it cools down !)

## 3. 

(a) QM:
$$ E = \hbar \omega (q + \frac{N}{2}) \quad || \quad q = \sum_i n_i, \ n_i = 0 \dots \infty $$

multiplicity
$$ \Omega(N, q) = \binom{q+N-1}{q} = \frac{(q+N-1)!}{q!(N-1)!} $$

for large $q, N$,
$$ \ln \Omega(N, q) \approx (q+N) \ln(q+N) - q \ln q - N \ln N $$
$$ S = k_B \ln \Omega = k_B [(q+N)\ln(q+N) - q \ln q - N \ln N] $$

---

(b) For $q \gg N$ (high-T limit)
<div align="right">using $\ln(1+x) \approx x$ for $x \ll 1$</div>

$$ S \approx k_B \left[ (q+N) \cdot (\ln q + \frac{N}{q}) - q \ln q - N \ln N \right] $$
$$ = k_B \left[ N \ln \frac{q}{N} + N \right] $$

$$ \therefore \quad S \simeq N k_B \left[ \ln \frac{q}{N} + 1 \right] $$

$$ \Rightarrow \quad \frac{1}{T} = \left(\frac{\partial S}{\partial E}\right)_N = \frac{N k_B}{E} \quad || \quad E \approx \hbar \omega q \text{ for } q \gg N $$

$$ \therefore \quad E = N k_B T $$

then
$$ C_v = \left(\frac{\partial E}{\partial T}\right)_N = N k_B $$

---

(c) CM:
$$ E = \sum_{i=1}^N \left( \frac{p_i^2}{2m} + \frac{1}{2} m \omega^2 x_i^2 \right) $$

$$ \Omega(E, N) = \frac{1}{h^N} \int_{\sum \frac{p_i^2}{2m} + \frac{1}{2} m \omega^2 x_i^2 = E} dx_1 dx_2 \dots dx_N \ dp_1 dp_2 \dots dp_N $$

> * No $\frac{1}{N!}$
> $\because$ oscillators are distinguishable.

---

change of variables.
$$ z_i = \frac{p_i}{\sqrt{2m}} \quad \text{for } i = 1 \dots N $$
$$ \left( z_{i+N} = \sqrt{\frac{m\omega^2}{2}} x_i \right. $$

$$ \Rightarrow \quad E = \sum_{i=1}^{2N} z_i^2 $$

$$ \Omega(E,N) = \frac{1}{h^N} \left( \frac{2}{m\omega^2} \right)^{\frac{N}{2}} \cdot (2m)^{\frac{N}{2}} \int_{\sum_{\mu=1}^{2N} z_\mu^2 = E} dz_1 dz_2 \dots dz_{2N} $$

$$ = \left( \frac{2}{h\omega} \right)^N a_{2N}(\sqrt{E}) $$

$$ = \left( \frac{2}{h\omega} \right)^N \cdot \frac{2\pi^N}{(N-1)!} E^{\frac{2N-1}{2}} $$

$$ S(E,N) = k_B \ln \Omega(E,N) \approx N k_B \ln E + O(N) + \dots $$

$$ \Rightarrow \quad \frac{1}{T} = \left( \frac{\partial S}{\partial E} \right)_N = \frac{N k_B}{E} \quad \Rightarrow \quad \left[ \begin{aligned} E &= N k_B T \\ C_N &= N k_B \end{aligned} \right. \quad ! $$

## 4. 
(i) $u = U/V \equiv u(T)$, (ii) $P = \frac{1}{3}u(T)$ (iii) $\mu = 0$

(a) $TdS = dU + PdV \leftarrow$ 1st and 2nd laws

$$ dU = \left( \frac{\partial U}{\partial T} \right)_V dT + \left( \frac{\partial U}{\partial V} \right)_T dV \qquad \downarrow \quad U = uV $$

$$ = V \frac{\partial u}{\partial T} dT + u dV $$

$$ \Rightarrow \quad dS = \frac{V}{T} \frac{\partial u}{\partial T} dT + \frac{4}{3} \frac{u}{T} dV $$

Maxwell relation :
$$ \frac{\partial}{\partial V} \left( \frac{V}{T} \frac{\partial u}{\partial T} \right) = \frac{\partial}{\partial T} \left( \frac{4}{3} \frac{u}{T} \right) $$

---

$$
\Rightarrow \frac{1}{T} \frac{\partial U}{\partial T} = \frac{4}{3} \left( \frac{1}{T} \frac{\partial U}{\partial T} - \frac{U}{T^2} \right)
$$

$$
\frac{1}{3} \cdot \frac{1}{T} \frac{\partial U}{\partial T} = \frac{4}{3} \frac{U}{T^2} \Rightarrow \frac{1}{u} dU = \frac{4}{T} dT
$$

$$
\Rightarrow \underline{\underline{u(T) = A T^4}}
$$

---

(b) $F(T,V) = -\frac{1}{3} \sigma V T^4$

$$
\rightarrow -S = \left(\frac{\partial F}{\partial T}\right)_{V,N} = -\frac{4}{3} \sigma V T^3
$$

Thus, $U = F + TS = -\frac{1}{3} \sigma V T^4 + \frac{4}{3} \sigma V T^4 = \sigma V T^4$

$$
\Rightarrow A = \sigma \quad \therefore \underline{u(T) = \sigma T^4}
$$

---

(c) $P \uparrow$

**Graph Description:**
A PV diagram showing a cycle $a \rightarrow b \rightarrow c \rightarrow d \rightarrow a$.
*   **y-axis:** $P_H$, $P_L$
*   **x-axis:** $V_1$, $V_4$, $V_2$, $V_3$
*   **Path $a \rightarrow b$:** $P = \text{const}$ (at $P_H$)
*   **Path $b \rightarrow c$:** $PV^{4/3} = \text{const}$ (Expansion)
*   **Path $c \rightarrow d$:** $P = \text{const}$ (at $P_L$)
*   **Path $d \rightarrow a$:** $PV^{4/3} = \text{const}$ (Compression)

**Formulas (Right side of graph):**

$$
P = \frac{1}{3} \sigma T^4
$$

$\downarrow$

Isothermal:
$$
P_{H,L} = \frac{1}{3} \sigma T_{H,L}^4
$$

$$
S = \frac{4}{3} \sigma V T^3
$$

Adiabatic:
$$
VT^3 = \text{const.}
$$
$$
\rightarrow V \cdot P^{3/4} = \text{const}
$$
$$
\rightarrow P \propto V^{-4/3}
$$

---

(d) $a \rightarrow b$: $Q_H = \Delta U + P \Delta V$

$$
= \frac{4}{3} \sigma T_H^4 (V_2 - V_1)
$$

$c \rightarrow d$: $Q_L = \frac{4}{3} \sigma T_L^4 (V_3 - V_4)$

$$
= \frac{4}{3} \sigma T_L T_H^3 (V_2 - V_1)
$$

$$
e = \frac{Q_H - Q_L}{Q_H} = \frac{T_H - T_L}{T_H} \quad \#
$$

## 5. 
(a)

**Graph (P vs T):**
*   **Y-axis:** P
*   **X-axis:** T
*   **Curve:** A curve rising from left to right.
*   **Labels:** Region $l$ (above/left), Region $g$ (below/right).
*   **Annotation:** $d\mu_l = d\mu_g$ along the phase coexistence curve.

$$ G = \mu N $$

$$ \rightarrow dG_l = dG_g \rightarrow -S_l dT + V_l dP = -S_g dT + V_g dP $$

$$ \therefore \frac{dP}{dT}\bigg|_{coexist} = \frac{S_g - S_l}{V_g - V_l} > 0 \quad (\because S_g > S_l, \ V_g > V_l) $$

---

**(b)**

**Graph (P vs V):**
*   **Y-axis:** P
*   **X-axis:** V
*   **Curves:** Three isotherms shown.
    *   **High T:** Hyperbolic shape.
    *   **$T_c$:** Critical isotherm passing through an inflection point (marked with a dot).
    *   **Low T:** Wavy curve with a dashed horizontal line indicating phase transition.
*   **Text:** at $T = T_c, \ P = P_c, \ V = V_c$

**Conditions:**
$$ \frac{\partial P}{\partial V} = 0 \quad , \quad \frac{\partial^2 P}{\partial V^2} = 0 $$

**EOS of vdW:**
$$ P = \frac{N k_B T}{V - Nb} - \frac{a N^2}{V^2} $$

**Derivatives:**
$$ \frac{\partial P}{\partial V} = -\frac{N k_B T}{(V-Nb)^2} + \frac{2 a N^2}{V^3} $$

$$ \frac{\partial^2 P}{\partial V^2} = \frac{2 N k_B T}{(V-Nb)^3} - \frac{6 a N^2}{V^4} $$

**Solving:**
$$ \Rightarrow \frac{2}{V-Nb} = \frac{3}{V} $$
*(Note: Derived from equating terms)*

$$ \Rightarrow 2V = 3V - 3Nb $$
$$ \Rightarrow V = 3Nb $$

$$ \therefore V_c = 3Nb \Rightarrow k_B T_c = \frac{8a}{27b} \Rightarrow P_c = \frac{a}{27b^2} $$

---

**(c)**

$$ dF = -S dT - P dV $$
*(Note: $-S dT$ is crossed out with a $0$, annotated "for a given T")*

$$ dF = \left( -\frac{N k_B T}{V-Nb} + \frac{a N^2}{V^2} \right) dV = \left(\frac{\partial F}{\partial V}\right)_T $$

$$ F = -N k_B T \ln[V-Nb] - \frac{a N^2}{V} + C(T,N) $$

$$ \Rightarrow G = F + PV = -N k_B T \ln(V-Nb) - \frac{a N^2}{V} + PV + C(T,N) $$

---

Let $v = V/V_c$ , $p = P/P_c$ , $t = T/T_c$

$$G = - N k_B T_c t \cdot \ln (V_c v - Nb) - \frac{aN^2}{V_c v} + P_c V_c pv$$
$$+ \ C(T, N)$$

$$g = \frac{8G}{3 N k_B T_c} = - \frac{8}{3} t \ln (3v - 1) - \frac{8 a N^2}{3 N k_B T_c V_c} \cdot \frac{1}{v}$$
$$+ \frac{8 P_c V_c}{3 N k_B T_c} pv + C'(T, N)$$

$$\frac{8 a N^2}{3 N k_B T_c V_c} = \frac{8 a N}{3 \cdot \frac{8a}{27b} \cdot 3Nb} = 3$$

$$\frac{8 P_c V_c}{3 N k_B T_c} = \frac{8 \cdot \frac{a}{27b^2} \cdot 3Nb}{3 N \cdot \frac{8a}{27b}} = 1$$

$$\Rightarrow g = - \frac{3}{v} - \frac{8}{3} t \ln(3v - 1) + pv + C'(T,N)$$

***

$1 - 2$ : stable, gas; $2 - 3$ : (meta) stable, gas

$3 - 4 - 5$ : unstable $\left( \frac{\partial^2 G}{\partial P^2} \bigg|_{T,N} > 0 \right)$

$\qquad \qquad \qquad \qquad \llcorner = \frac{\partial V}{\partial P} \bigg|_{T,N} = - V \kappa_T < 0$
$\qquad \qquad \qquad \qquad \qquad \qquad \qquad \qquad$ by 2nd law!

$5 - 6$ : (meta) stable, liq.

$6 - 7$ : stable, liq.

Stability condition

---

Maxwell construction.

$$ \oint dG = 0 \quad \Rightarrow \quad \int_{2\rightarrow3\rightarrow4\rightarrow5\rightarrow6} V dP = 0 $$

<table border="0" style="width:100%">
  <tr>
    <td style="width:40%">
      <!-- Interpretation of Graph 1 -->
      <strong>Graph 1: P-V Diagram (Rotated)</strong><br>
      <ul>
        <li>Y-axis: V (implied)</li>
        <li>X-axis: P</li>
        <li>Curve points: 2, 3, 4, 5, 6</li>
        <li>Areas: A (shaded region 3-4), B (shaded region 4-5)</li>
        <li>Dashed vertical line at P<sub>v</sub></li>
      </ul>
    </td>
    <td style="width:60%">
      $$ \int_{2\rightarrow3} VdP - \int_{4\rightarrow3} VdP = \int_{5\rightarrow4} VdP - \int_{5\rightarrow6} VdP $$
      <br>
      $$ (\text{area } A) = (\text{area } B) $$
    </td>
  </tr>
</table>

<table border="0" style="width:100%">
  <tr>
    <td style="width:40%">
      <!-- Interpretation of Graph 2 -->
      <strong>Graph 2: P-v Diagram</strong><br>
      <ul>
        <li>Y-axis: P, intercept at P<sub>v</sub></li>
        <li>X-axis: v, intercepts at v<sub>e</sub>, v<sub>g</sub></li>
        <li>Curve: Van der Waals loop</li>
        <li>Area A: Region above P<sub>v</sub></li>
        <li>Area B: Region below P<sub>v</sub></li>
      </ul>
    </td>
    <td style="width:60%">
      $$ A - B $$
      <br>
      $$ = \text{[Curve Area]} - \text{[Rectangle Area]} $$
      <br>
      $$ = \int_{v_e}^{v_g} p \, dv - P_v (v_g - v_e) $$
    </td>
  </tr>
</table>

$$ \Rightarrow \quad P_v (v_g - v_e) - \int_{v_e}^{v_g} p(v) \, dv = 0 $$